lemmas.v
@@ -1,6 +1,6 @@
 (* Lemmas on various topics. *)
 
-Require Import Utf8 List Lia.
+Require Import Utf8 PeanoNat List Lia.
 From larith Require Import tactics notations.
 Import ListNotations.
 
@@ -49,6 +49,12 @@ Proof.
 now induction l.
 Qed.
 
+Lemma list_prod_single {X Y} (x : X) (y : Y) :
+  [(x, y)] = list_prod [x] [y].
+Proof.
+easy.
+Qed.
+
 Lemma list_singleton {X} (l : list X) :
   length l = 1 -> ∃x, l = [x].
 Proof.
@@ -56,10 +62,81 @@ intros. destruct l. easy. destruct l.
 now exists x. easy.
 Qed.
 
-Lemma in_singleton {X} (x x' : X) :
-  In x [x'] -> x = x'.
+(* Construct a powerset. *)
+Theorem list_powerset {X} (l : list X) :
+  (∀x y : X, {x = y} + {x ≠ y}) ->
+  Σ L, length L = 2^length l /\
+  ∀s, (∀x, In x s -> In x l) <->
+  ∃t, In t L /\ ∀x, In x s <-> In x t.
 Proof.
-intros H; now inv H.
+intros dec; induction l.
+- exists [[]]; repeat split; simpl.
+  + intros H; exists []; split. now left.
+    split; intros. exfalso; eapply H, H0. easy.
+  + intros [t [H1 H2]]. destruct H1.
+    subst; intros. now apply H2 in H. easy.
+- destruct IHl as [L [L_len HL]].
+  exists (L ++ map (cons a) L); repeat split.
+  + rewrite app_length, map_length, L_len; simpl; lia.
+  + intros Hs; pose(s' := remove dec a s).
+    destruct (proj1 (HL s')) as [t Ht].
+    intros. apply in_remove in H as [H1 H2].
+    apply Hs in H1; inv H1; easy.
+    destruct (in_dec dec a s).
+    * exists (a :: t); split. apply in_app_iff; right.
+      apply in_map_iff; now exists t.
+      intros; split; intros. destruct (dec x a).
+      subst; apply in_eq. eapply in_cons, Ht. now apply in_in_remove.
+      inv H. apply Ht in H0. eapply in_remove, H0.
+    * exists t; split. apply in_app_iff; left. easy.
+      eapply notin_remove in n; rewrite <-n; apply Ht.
+  + intros [t [H1 H2]]. apply in_app_or in H1 as [H1|H1]; intros.
+    * eapply in_cons, HL. 2: apply H. now exists t.
+    * apply in_map_iff in H1 as [t' [H1a H1b]]; subst.
+      apply H2 in H; inv H. apply in_eq. apply in_cons.
+      eapply HL. 2: apply H0. now exists t'.
+Qed.
+
+Section Witness_list.
+
+Variable X Y : Type.
+Variable R : X -> Y -> Prop.
+Hypothesis ex : ∀x, ∃y : Y, R x y.
+
+Theorem witness_list xs :
+  ∃ys, Forall2 R xs ys.
+Proof.
+induction xs. now exists [].
+destruct (ex a) as [y Hy];
+destruct (IHxs) as [ys H].
+exists (y :: ys); now apply Forall2_cons.
+Qed.
+
+Theorem Forall2_in_l xs ys x :
+  In x xs -> Forall2 R xs ys -> ∃y, In y ys /\ R x y.
+Proof.
+revert ys; induction xs; simpl; intros. easy.
+destruct ys; simpl in *. easy. inv H0; destruct H.
+- subst; exists y; split. apply in_eq. easy.
+- eapply IHxs in H as [y' Hy']. 2: apply H6.
+  exists y'; split. now right. easy.
+Qed.
+
+Theorem Forall2_swap xs ys :
+  Forall2 R xs ys -> Forall2 (λ y x, R x y) ys xs.
+Proof.
+revert ys; induction xs; destruct ys; simpl; intros. 1-3: easy.
+inv H; apply Forall2_cons. easy. apply IHxs, H5.
+Qed.
+
+End Witness_list.
+
+Corollary Forall2_in_r {X Y} (xs : list X) (ys : list Y) R y :
+  In y ys -> Forall2 R xs ys -> ∃x, In x xs /\ R x y.
+Proof.
+intros Hy H; apply Forall2_swap in H.
+eapply Forall2_in_l in H as [x Hx].
+exists x; apply Hx. easy.
 Qed.
 
 Section Option_list_filtering.
